Forgot to do update-gold.

internal/examples/append_log/append_log.gold.v
@@ -71,12 +71,22 @@ Theorem Open_t: ⊢ Open : (unitT -> struct.ptrT Log.S).
 Proof. typecheck. Qed.
 Hint Resolve Open_t : types.
 
-Definition Log__Get: val :=
-  rec: "Log__Get" "log" "i" :=
+Definition Log__get: val :=
+  rec: "Log__get" "log" "i" :=
     let: "sz" := struct.loadF Log.S "sz" "log" in
     (if: "i" < "sz"
     then (disk.Read (#1 + "i"), #true)
     else (slice.nil, #false)).
+Theorem Log__get_t: ⊢ Log__get : (struct.ptrT Log.S -> uint64T -> (disk.blockT * boolT)).
+Proof. typecheck. Qed.
+Hint Resolve Log__get_t : types.
+
+Definition Log__Get: val :=
+  rec: "Log__Get" "log" "i" :=
+    lock.acquire (struct.loadF Log.S "m" "log");;
+    let: ("v", "b") := Log__get "log" "i" in
+    lock.release (struct.loadF Log.S "m" "log");;
+    ("v", "b").
 Theorem Log__Get_t: ⊢ Log__Get : (struct.ptrT Log.S -> uint64T -> (disk.blockT * boolT)).
 Proof. typecheck. Qed.
 Hint Resolve Log__Get_t : types.
@@ -89,8 +99,8 @@ Theorem writeAll_t: ⊢ writeAll : (slice.T disk.blockT -> uint64T -> unitT).
 Proof. typecheck. Qed.
 Hint Resolve writeAll_t : types.
 
-Definition Log__Append: val :=
-  rec: "Log__Append" "log" "bks" :=
+Definition Log__append: val :=
+  rec: "Log__append" "log" "bks" :=
     let: "sz" := struct.loadF Log.S "sz" "log" in
     (if: slice.len "bks" ≥ struct.loadF Log.S "diskSz" "log" - #1 - "sz"
     then #false
@@ -99,14 +109,34 @@ Definition Log__Append: val :=
       struct.storeF Log.S "sz" "log" (struct.loadF Log.S "sz" "log" + slice.len "bks");;
       Log__writeHdr "log";;
       #true).
+Theorem Log__append_t: ⊢ Log__append : (struct.ptrT Log.S -> slice.T disk.blockT -> boolT).
+Proof. typecheck. Qed.
+Hint Resolve Log__append_t : types.
+
+Definition Log__Append: val :=
+  rec: "Log__Append" "log" "bks" :=
+    lock.acquire (struct.loadF Log.S "m" "log");;
+    let: "b" := Log__append "log" "bks" in
+    lock.release (struct.loadF Log.S "m" "log");;
+    "b".
 Theorem Log__Append_t: ⊢ Log__Append : (struct.ptrT Log.S -> slice.T disk.blockT -> boolT).
 Proof. typecheck. Qed.
 Hint Resolve Log__Append_t : types.
 
-Definition Log__Reset: val :=
-  rec: "Log__Reset" "log" :=
+Definition Log__reset: val :=
+  rec: "Log__reset" "log" :=
     struct.storeF Log.S "sz" "log" #0;;
     Log__writeHdr "log".
+Theorem Log__reset_t: ⊢ Log__reset : (struct.ptrT Log.S -> unitT).
+Proof. typecheck. Qed.
+Hint Resolve Log__reset_t : types.
+
+Definition Log__Reset: val :=
+  rec: "Log__Reset" "log" :=
+    lock.acquire (struct.loadF Log.S "m" "log");;
+    Log__writeHdr "log";;
+    Log__reset "log";;
+    lock.release (struct.loadF Log.S "m" "log").
 Theorem Log__Reset_t: ⊢ Log__Reset : (struct.ptrT Log.S -> unitT).
 Proof. typecheck. Qed.
 Hint Resolve Log__Reset_t : types.
